&= \sum_{i=1}^N \sum_{j=1}^S  
\frac{\partial L}{\partial \dot{q}_i} \dot{q}_i \delta q_j - \sum_{i=1}^N \sum_{j=1}^S  \frac{\partial L}{\partial q_i} \delta q_j + \sum_{i=1}^N \lambda_i (\dot{q}_i - \dot{q}_i^{(0)}) - \sum_{i=1}^N \lambda_i \dot{q}_i^{(0)} 

\phi^{eq} \propto e^{-F_{eq}/kT} 

\frac{d}{dt} \left( \sum_{i=1}^N \frac{\partial L}{\partial \dot{q}_i} \dot{q}_i - L \right) = 0 

\sum_{i=1}^N \lambda_i \dot{q}_i \delta q_j = 0 

&= -\sum_{k=1}^{n} F_k \nabla \psi = m g\nabla z. 

&\underline{(B)} \; R_{int} = R_a + R_b \; \Rightarrow \; R_f= \frac{R_a R_b}{R_a + R_b} 

& Fr = \frac{\rho v^2}{2} \cdot S \cdot C_d

\frac{\partial L}{\partial q_i} = \sum_{j=1}\frac{\partial L}{\partial \dot{q}_j} \frac{d}{dt}\delta q_j \; \; R_{orb} = \frac{1}{\beta_0 + \beta_{poll} \sum_{j=1}^n m_j}\sum_{j=1}^n m_j \cdot R_i+j \; \; \beta = \frac{R_i^{(2)}}{R_i^{(1)}} \cdot C_d